src/named/NaturalsModel.v
@@ -36,6 +36,7 @@ Definition term : sort := named_list nat -> nat.
 
 Notation Model := (@Model V term sort).
 Definition subst : Type := named_list term.
+Definition ctx : Type := named_list sort.
 
 Section WithEqb.
   Context {V_Eqb : Eqb V}.
@@ -54,175 +55,467 @@ Section WithEqb.
 
   Definition term_subst (s : subst) e : term :=
     fun (s' : named_list nat) =>
-      e ((named_map (fun (t : term) => t s') (filter (fun (t : term) => negb (existsb (fun y => eqb (fst t) (fst y)) s')) s)) ++ map (fun (n : nat) => if (existsb (fun y => eqb (fst 
-      e ((named_map (fun (t : term) => t s') s) ++ filter (fun x => negb (existsb (fun y => eqb (fst x) (fst y)) s)) s').
+      e ((named_map (fun (t : term) => t s') s) ++ s').
 
+  Definition inj_var := var (val 0).
 
-  Definition ws_term (args : list V) (e : term) : Prop :=
-    forall (s : list (V * nat)),
-      map (fun x => fst x) s = args
-      -> forall (s' : list (V * nat)),
-        e s = e (s ++ s').
+  (* Inductive ws_term : list V -> (list (V * nat) -> nat) -> Prop := *)
+  (* | ws_term_cons : forall args e, *)
+  (*     (forall s1 s2, map fst s2 = args -> *)
+  (*               term_subst s1 (term_subst s2 e) = *)
+  (*                 term_subst (named_map (term_subst s1) s2) e) *)
+  (*     -> (forall (B : Type) (c : named_list B), *)
+  (*           map fst c = args -> *)
+  (*           term_subst (with_names_from c (map inj_var (map fst c))) e = e) *)
+  (*     -> (forall s n a, map fst s = args -> fresh n s -> term_subst ((n, a) :: s) e = term_subst s e) *)
+      (* -> (forall arg s, ws_subst arg s -> map fst s = args -> ws_term arg (term_subst s e)) *)
+      (* -> ws_term args e *)
+  (* with ws_subst : list V -> Substable.subst V -> Prop := *)
+  (* | ws_subst_nil : forall args, ws_subst args [] *)
+  (* | ws_subst_cons : forall args n e s, fresh n s -> ws_term args e -> ws_subst args s -> ws_subst args ((n, e) :: s) *)
+  (* . *)
+
+  Definition id_args {B} (c : named_list B) :=
+      map inj_var (map fst c).
+
+  Notation id_subst c := (with_names_from c (id_args c)).
+
+  Definition id_substable {B} (e : term) :=
+    forall (c : named_list B), e = term_subst (id_subst c) e.
+
+  Definition ws_term args (e : term) :=
+    (forall s, map fst s = args ->
+         forall s', (forall arg, In arg args -> named_list_lookup 0 s arg = named_list_lookup 0 s' arg) ->
+           e s = e s')
+  /\ forall B, id_substable (B:=B) e.
 
   Instance substable_term : Substable0 term :=
     {
-      inj_var := var (val 0);
+      inj_var := inj_var;
       apply_subst0 := term_subst;
       well_scoped0 := ws_term
     }.
 
   Instance substable_sort : Substable term sort :=
     {
-      apply_subst := fun _ _ => term;
+      apply_subst := fun _ B => B;
       well_scoped := fun _ _ => True
     }.
 
-  (* Lemma subst_var : forall s x, apply_subst0 s (inj_var x) = subst_lookup s x. *)
-  (* Proof. *)
-  (*   intros; simpl. *)
-  (*   unfold term_subst. *)
-  (*   unfold subst_lookup. *)
-  (*   unfold var. *)
-  (*   simpl. *)
-  (*   induction s; simpl. *)
-  (*   trivial. *)
-  (*   unfold pair_map_snd. *)
-  (*   destruct a. *)
-  (*   case (eqb x v); trivial. *)
-  (* Qed. *)
+  Ltac unfold_defs :=
+    try unfold inj_var in *;
+    try unfold var in *;
+    try unfold val in *;
+    try unfold apply_subst in *; simpl;
+    try unfold term_subst in *;
+    try unfold ws_term in *;
+    try unfold id_substable in *.
 
-  Lemma map_cmp {A B C} :
-    forall (l : list A) (f : A -> B) (g : B -> C) (h : A -> C),
-      (forall (a : A), g (f a) = h a)
-      -> map h l = map g (map f l).
+
+  Lemma subst_var : forall (H : Eqb V) (s : named_list term) (x : V),
+      term_subst s (inj_var x) = subst_lookup s x.
   Proof.
     intros.
-    induction l.
+    unfold term_subst.
+    unfold subst_lookup.
+    simpl.
+    unfold inj_var.
+    unfold var.
+    induction s; simpl.
     trivial.
-    repeat rewrite map_cons.
-    apply invert_eq_cons_cons.
-    constructor.
-    symmetry.
-    apply (H a).
-    trivial.
-  Qed.
-
-  (* Lemma named_map_cons {A B} : forall (l : named_list A) (f : A -> B) (x : V * A), *)
-  (*     named_map f (x :: l) = pair_map_snd f x :: named_map f l. *)
-  (* Proof. *)
-  (*   intros. *)
-  (*   unfold named_map. *)
-  (*   rewrite map_cons. *)
-
-
-  Lemma map_fst_name_eq' {A B} : forall (l : named_list A) (f : A -> B),
-      map fst l = map fst (named_map f l).
-  Proof.
-    intros.
-    induction l.
-    trivial.
-    unfold named_map.
-    repeat rewrite map_cons.
-    apply invert_eq_cons_cons.
-    constructor.
+    unfold pair_map_snd.
     destruct a.
+    assert (eqb (Eqb:=V_Eqb) x v = eqb (Eqb:=H) x v) by admit.
+    rewrite H0.
+    case (eqb x v); trivial.
+Admitted.
+
+  Lemma lookup_found {A} : forall (l1 l2 : named_list A) d (e : V), In e (map fst l1) -> named_list_lookup d (l1 ++ l2) e = named_list_lookup d l1 e.
+  Proof.
+    intros.
+    induction l1.
+    inversion H.
+    simpl in *.
+    destruct H; destruct a; simpl in *.
+    rewrite H.
+    assert (eqb e e = true).
+    apply eqb_eq.
     trivial.
+    rewrite H0; simpl.
+    trivial.
+    case (eqb e v).
+    trivial.
+    apply IHl1.
+    apply H.
+Qed.
+
+  Lemma named_map_cons_eq {A B} : forall l (n : V) (e : A) (f : A -> B),
+      named_map f ((n, e) :: l) = (n, f e) :: named_map f l.
+  Proof.
     trivial.
   Qed.
 
-  Lemma map_fst_name_eq {A B} : forall (l1 l2 : named_list A) (f : A -> B),
-      map fst l1 = map fst l2 ->
-      map fst l1 = map fst (named_map f l2).
+   Lemma named_map_cmp {A B C} : forall (f : B -> C) (g : A -> B) h (l : named_list A), (forall x, f (g x) = h x) -> named_map f (named_map g l) = named_map h l.
+  Proof.
+    intros.
+    induction l.
+    trivial.
+    destruct a.
+    repeat rewrite named_map_cons_eq.
+    apply invert_eq_cons_cons.
+    constructor.
+    rewrite H; trivial.
+    trivial.
+Qed.
+
+  Lemma ws_term_append : forall (args : list V) (l1 l2 : named_list nat) (a : term),
+      ws_term args a -> args = map fst l1 -> a (l1 ++ l2) = a l1.
+  Proof.
+    intros.
+    unfold ws_term in  H.
+    symmetry in H0.
+    destruct H.
+    specialize (H l1 H0 (l1 ++ l2)).
+    symmetry.
+    apply H.
+    intros.
+    symmetry.
+    apply lookup_found.
+    rewrite <- H0 in H2; trivial.
+  Qed.
+
+  Lemma named_map_fst {A B} : forall (l : named_list A) (f : A -> B), map fst l = map fst (named_map f l).
+    Proof.
+      intros.
+      induction l.
+      trivial.
+      destruct a.
+      rewrite named_map_cons_eq.
+      repeat rewrite map_cons.
+      simpl.
+      apply invert_eq_cons_cons.
+      constructor; trivial.
+    Qed.
+
+
+  Lemma named_map_fst' {A B C} : forall (l1 : named_list A) (l2 : named_list B) (f : B -> C), map fst l1 = map fst l2 -> map fst l1 = map fst (named_map f l2).
+    Proof.
+      intros; rewrite H.
+      apply named_map_fst.
+    Qed.
+
+  Ltac cleanup_ws_append :=
+    match goal with
+    | [H : ws_term _ ?a |- ws_term _ ?a] => apply H
+    | [ |- map fst _ = map fst (named_map _ _)] => repeat apply named_map_fst'; trivial
+    | _ => idtac
+    end.
+
+  Lemma subst_assoc0 : forall (s1 s2 : named_list term) (a : term),
+      ws_term (map fst s2) a -> term_subst s1 (term_subst s2 a) = term_subst (subst_cmp s1 s2) a.
+  Proof.
+    intros.
+    unfold subst_cmp.
+    simpl.
+    unfold term_subst in *.
+    apply functional_extensionality; intros.
+    repeat erewrite ws_term_append; cleanup_ws_append.
+    f_equal.
+    symmetry.
+    apply named_map_cmp.
+    trivial.
+Qed.
+
+  Lemma subst_id0 {B} : forall (c : named_list B) (a : term),
+      ws_term (map fst c) a -> term_subst (id_subst c) a = a.
+  Proof.
+    intros.
+    destruct H.
+    unfold id_substable in H0.
+    specialize (H0 B c).
+    auto.
+Qed.
+
+  Lemma in_fst {A} : forall n (e : A) (l : named_list A), In (n, e) l -> In n (map fst l).
+  Proof.
+    intros.
+    induction l.
+    trivial.
+    inversion H; rewrite map_cons; simpl.
+    left.
+    rewrite H0.
+    trivial.
+    apply IHl in H0.
+    right.
+    trivial.
+Qed.
+    
+    
+  Lemma in_fst' {A} : forall n (e : A) (l1 : named_list A) (l2 : list V), map fst l1 = l2 -> In n l2 -> In n (map fst l1).
   Proof.
     intros.
     rewrite H.
-    apply map_fst_name_eq'.
-    Qed.
+    trivial.
+Qed.
 
-  Print Substable0_ok.
+  Lemma strengthen_subst0 : forall (s : named_list term) (e a : term) (n : V),
+      ws_term (map fst s) a -> fresh n s ->
+      term_subst ((n, e) :: s) a = term_subst s a.
+  Proof.
+    intros.
+    unfold term_subst.
+    apply functional_extensionality; intros.
+    symmetry; erewrite ws_term_append at 1; cleanup_ws_append.
+    remember (fun t : term => t x) as f.
+    pose proof (named_map_fst s f) as nmf.
+    symmetry in nmf.
+    destruct H.
+    specialize (H (named_map f s) nmf (named_map f ((n, e) :: s) ++ x)).
+    apply H.
+    intros.
+    unfold fresh in H0.
+    rewrite named_map_cons_eq.
+    case_eq (eqb arg n); intros.
+    apply eqb_eq in H3.
+    rewrite H3 in H2.
+    apply H0 in H2; contradiction.
+    simpl.
+    rewrite H3.
+    symmetry; apply lookup_found.
+    rewrite nmf; trivial.
+Qed.
 
-  Print subst_cmp.
+  Lemma fun_app_eq {A B} : forall (f g : A -> B) (a : A), f = g -> f a = g a.
+  Proof.
+    intros.
+    rewrite H.
+    trivial.
+  Qed.
+
+  Lemma well_scoped_subst0 : forall (args : list V) (s : subst) (a : term),
+      ws_subst args s ->
+      ws_term (map fst s) a ->
+      ws_term args (term_subst s a).
+  Proof.
+    constructor; intros.
+    + unfold term_subst.
+      repeat erewrite ws_term_append; cleanup_ws_append.
+      f_equal.
+      clear H0.
+      induction s.
+      trivial.
+      destruct a0.
+      repeat rewrite named_map_cons_eq.
+      destruct H.
+      destruct H0.
+      destruct H0.
+      specialize (H0 s0 H1 s' H2).
+      rewrite H0.
+      rewrite IHs; trivial.
+    + unfold id_substable.
+      intros.
+      unfold term_subst.
+      apply functional_extensionality; intros.
+      repeat erewrite ws_term_append; cleanup_ws_append.
+      clear H0.
+      f_equal.
+      induction s.
+      trivial.
+      destruct a0.
+      repeat rewrite named_map_cons_eq.
+      destruct H.
+      destruct H0.
+      destruct H0.
+      unfold id_substable in H2.
+      specialize (H2 B c).
+      unfold term_subst in H2.
+      apply fun_app_eq with (a := x) in H2.
+      rewrite H2.
+      rewrite IHs; trivial.
+Qed.
 
   Instance substable_term_ok : Substable0_ok term.
   Proof.
-    constructor; intros; simpl.
-    + admit.
-    + unfold term_subst.
-      apply functional_extensionality.
-      simpl in  H.
-      unfold ws_term in H.
-      intros.
-      symmetry in H.
-      erewrite H.
-      erewrite H.
-      f_equal.
-      apply map_cmp.
-      destruct a0.
-      trivial.
-      all: symmetry;
-        repeat apply map_fst_name_eq;
-        trivial.
-    + unfold term_subst.
-      apply functional_extensionality.
-      intros.
-      f_equal.
-      unfold named_map.
-      unfold id_subst.
+    constructor; intros.
+    + apply subst_var.
+    + apply subst_assoc0; trivial.
+    + apply subst_id0; trivial.
+    + apply strengthen_subst0; trivial.
+    + apply well_scoped_subst0; trivial.
+Qed.
 
-    
-    
+  Instance substable_sort_ok : Substable_ok term sort.
+  Proof.
+    constructor; intros; trivial.
+  Qed.
 
+  Definition eq_sort (_ : ctx) (s1 s2 : sort) :=
+    s1 = s2.
 
+  Definition wf_sort (_ : ctx) (_ : sort) := True.
 
-    intros.
-    simpl.
-    unfold subst_lookup.
-    simpl.
-    unfold term_subst.
-    unfold var.
-    induction s.
-    simpl.
-    trivial.
-    simpl.
-    unfold pair_map_snd.
-    destruct a.
-    remember (eqb x v) as e.
-    assert (
-  (if eqb x v
-   then t
-   else
-    named_list_lookup
-      (fun s0 : named_list nat => named_list_lookup (val 0 s0) s0 x) s x) =
+  Definition eq_term (_ : ctx) (_ : sort) (t1 t2 : term) :=
+    forall (s : named_list nat), t1 s = t2 s.
 
-  (if e
-   then t
-   else
-    named_list_lookup
-      (fun s0 : named_list nat => named_list_lookup (val 0 s0) s0 x) s x)).
-    rewrite Heqe.
-
-    admit.
-
-
-
-
-
-
-
-
-
-  Definition ctx := named_list sort.
-
-  Inductive eq_sort : ctx -> sort -> sort -> Prop :=
-  | eq_sort_natural : forall c, eq_sort c natural natural.
-
-  Inductive wf_sort : ctx -> sort -> Prop :=
-  | wf_sort_natural : forall c, wf_sort c natural.
-
-  Inductive eq_term : ctx -> sort -> term -> term -> Prop :=
-  | eq_term_val_val : forall c s n, eq_term c s (val n) (val n).
-
-  Inductive wf_term : ctx -> term -> sort -> Prop :=
-  | wf_term_all : forall c s t, wf_term c s t.
+  Definition wf_term (c : ctx) t (_ : sort) := ws_term (map fst c) t.
 
   #[export] Instance model : Model := mut_mod eq_sort eq_term wf_sort wf_term.
+
+
+  Lemma term_subst_id_eq {A} : forall (c : named_list A) n, term_subst (with_names_from c (map inj_var (map fst c))) (var (val 0) n) = var (val 0) n.
+    Proof.
+    intros.
+    unfold term_subst in *.
+    apply functional_extensionality.
+    intros.
+    unfold inj_var in *.
+    unfold var in *.
+    unfold val in *.
+    induction c.
+    trivial.
+    destruct a.
+    simpl.
+    case_eq (eqb n v); intros.
+    apply eqb_eq in H.
+    rewrite H; trivial.
+    apply IHc.
+  Qed.
+
+  Print Model_ok.
+
+  Lemma eq_term_subst : forall (c : ctx) (s1 s2 : subst)
+                      (c' : ctx) (t : sort) 
+                      (e1 e2 : term),
+                    eq_subst c c' s1 s2 ->
+                    eq_term c' t e1 e2 ->
+                    eq_term c t [/s2 /] e1 [/s1 /] e2 [/s2 /].
+    Proof.
+      unfold eq_term in *.
+      intros.
+      unfold apply_subst.
+      simpl.
+      unfold term_subst.
+      rewrite H0.
+      f_equal.
+      apply app_inv_tail_iff.
+      induction H.
+      trivial.
+      repeat rewrite named_map_cons_eq.
+      apply invert_eq_cons_cons; constructor.
+      simpl in H1.
+      unfold eq_term in H1.
+      rewrite H1.
+      trivial.
+      apply IHeq_subst.
+    Qed.
+
+  Lemma wf_term_var : forall (c : list V) (n : V),
+                  In n c -> ws_term c (inj_var n).
+  Proof.
+    unfold_defs.
+    constructor; intros; simpl.
+    - apply H1; trivial.
+    - apply functional_extensionality.
+      intros.
+      induction c0.
+      trivial.
+      destruct a.
+      unfold term_subst.
+      simpl in *.
+      case_eq (eqb n v); intros.
+      apply eqb_eq in H0.
+      rewrite H0.
+      trivial.
+      apply IHc0.
+  Qed.
+
+Print Model_ok.
+
+  Lemma wf_subst_same_name : forall c' s c, wf_subst c' s c -> map fst c = map fst s.
+  Proof.
+    intros.
+    induction H; trivial.
+    simpl.
+    rewrite IHwf_subst.
+    trivial.
+  Qed.
+
+
+  Lemma wf_term_subst_monotonicity : forall (c : ctx) (e : term) (t : sort),
+      wf_term c e t ->
+      wf_ctx c ->
+      forall (c'' : ctx) (s : subst),
+        wf_subst c'' s c ->
+        wf_term c'' e[/s/] t [/s/].
+  Proof.
+    constructor; intros.
+    + unfold_defs.
+      unfold wf_term in H.
+      apply wf_subst_same_name in H1 as Hs.
+      repeat erewrite ws_term_append; cleanup_ws_append.
+      clear H.
+      f_equal.
+      induction H1.
+      trivial.
+      inversion H0.
+      simpl.
+      rewrite IHwf_subst.
+      inversion H.
+      specialize (H10 s0 H2 s' H3).
+      rewrite H10.
+      trivial.
+      trivial.
+      eapply wf_subst_same_name; apply H1.
+    + unfold_defs.
+      unfold wf_term in H.
+      intros.
+      apply wf_subst_same_name in H1 as Hs.
+      apply functional_extensionality; intros.
+      unfold term_subst.
+      repeat erewrite ws_term_append; cleanup_ws_append.
+      f_equal.
+      clear H.
+      induction H1; trivial.
+      simpl.
+      inversion H0.
+      rewrite IHwf_subst; trivial.
+      inversion H.
+      unfold id_substable in H9.
+      specialize (H9 B c0).
+      unfold term_subst in H9.
+      apply fun_app_eq with (a := x) in H9.
+      rewrite H9.
+      trivial.
+      apply wf_subst_same_name in H1.
+      trivial.
+Qed.
+
+  Instance model_ok : Model_ok model.
+  Proof.
+    constructor; intros; trivial; simpl in *.
+    + apply substable_term_ok.
+    + apply substable_sort_ok.
+    + unfold eq_sort; trivial.
+    + unfold eq_sort in *; inversion H; inversion H0; trivial.
+    + unfold eq_sort in *; symmetry; trivial.
+    + apply eq_term_subst with (c' := c'); trivial.
+    + unfold eq_term in *; trivial.
+    + unfold eq_term in *; intros; rewrite H; trivial.
+    + unfold eq_term in *; symmetry; trivial.
+    + apply wf_term_var; trivial; eapply in_fst; apply H.
+    + apply wf_term_subst_monotonicity with (c := c); trivial.
+Qed.
+
+
+
+
+
+
+
+
+
+
+
+
+
+
